set fold verified

Set_Graphs/Graph_Algorithms/Set_Map_Fold.thy
@@ -6,14 +6,14 @@ locale set_fold_locale =
 imp_set_iterate where is_set = is_set and it_next = it_next +
 imp_set_ins where ins = ins and is_set = is_set +
 imp_set_empty where empty = empty and is_set = is_set
-for is_set :: "nat set \<Rightarrow> 'simpl \<Rightarrow> assn" 
-and ins :: "nat \<Rightarrow> 'simpl \<Rightarrow> 'simpl Heap"
+for is_set :: "'a set \<Rightarrow> 'simpl \<Rightarrow> assn" 
+and ins :: "'a \<Rightarrow> 'simpl \<Rightarrow> 'simpl Heap"
 and empty :: "'simpl Heap"
-and it_next :: "'it \<Rightarrow> (nat \<times> 'it) Heap"
+and it_next :: "'it \<Rightarrow> ('a \<times> 'it) Heap"
 begin
 
 
-partial_function (heap) set_fold_loop ::"'it \<Rightarrow>(nat => nat => nat Heap) \<Rightarrow> nat  \<Rightarrow> nat Heap"
+partial_function (heap) set_fold_loop ::"'it \<Rightarrow>('a => 'b => 'b Heap) \<Rightarrow> 'b  \<Rightarrow> 'b Heap"
   where
 "set_fold_loop it f acc = 
   (do {b <- it_has_next it;
@@ -24,11 +24,131 @@ partial_function (heap) set_fold_loop ::"'it \<Rightarrow>(nat => nat => nat Hea
            set_fold_loop it' f acc'
        }})"
 
+definition "simple_prog f acc it = 
+  do {
+         (x, it') <- it_next it;
+          acc' <- f x acc;
+          return acc'}"
+
+lemma it_next_rule_empty_in_ass:
+    "<is_it s p s' it  * \<up> (s' \<noteq> {})> 
+      it_next it 
+    <\<lambda>(a,it'). is_it s p (s' - {a}) it' * \<up>(a \<in> s')>"
+  by sep_auto
+
+lemma 
+assumes "\<And> x y. <true>fimpl x y <\<lambda> r. \<up> (r = f x y)>"
+shows "<is_it S Simpl S' it * \<up> (S' \<noteq> {})> simple_prog fimpl acc it
+ <\<lambda>r. \<exists>\<^sub>A x. \<up> (x \<in> S' \<and> r = f x acc)  * is_set S Simpl>"
+  unfolding simple_prog_def
+  apply(rule ht_bind)
+   apply(rule it_next_rule_empty_in_ass)
+  subgoal for x
+    apply(cases x)
+    subgoal for x it
+      apply simp
+      apply(rule ht_cons_post[of _ _ 
+           "\<lambda>r. \<up> ( r = f x acc) * (\<up> (x \<in> S')* is_set S Simpl)"])
+        apply(rule ht_cons_pre[OF _ ht_frame[OF assms[of x acc]]])
+        by(sep_auto intro: quit_iteration)
+      done
+    done
+
 definition "set_fold Simpl= (\<lambda> f acc. 
          do {it_init <- it_init Simpl;
              set_fold_loop it_init f acc})"
 
 lemmas [code] = set_fold_loop.simps set_fold_def
+
+lemma weaken_conditions_and_frame:
+  assumes "P1 \<Longrightarrow>\<^sub>A P1'*P"
+          "\<And> r. P1'*Q r \<Longrightarrow>\<^sub>A P1'' r"
+          "<P>c<Q>" 
+     shows "<P1>c<P1''>"
+  apply(rule ht_cons_prec[of P1 "P*P1'" "\<lambda> r. Q r*P1'" P1'' c ])
+  using assms by(sep_auto intro: fr_refl ent_star_mono simp: star_aci(2))
+
+lemma pure_assn_adjunct_concl:
+"P \<Longrightarrow>\<^sub>A \<up>Q1*true \<Longrightarrow> P \<Longrightarrow>\<^sub>A Q2 \<Longrightarrow> P \<Longrightarrow>\<^sub>A \<up> Q1*Q2"
+  by sep_auto
+
+lemma pure_assn_adjunct_prec:
+"\<lbrakk> P1 \<Longrightarrow> P2 \<Longrightarrow>\<^sub>A Q\<rbrakk> \<Longrightarrow> \<up>P1*P2 \<Longrightarrow>\<^sub>A Q"
+"\<lbrakk> P1 \<Longrightarrow> P2 \<Longrightarrow>\<^sub>A Q\<rbrakk> \<Longrightarrow> P2*\<up>P1 \<Longrightarrow>\<^sub>A Q"
+  by sep_auto
+
+lemma pure_conclI: 
+  "Q \<Longrightarrow> P \<Longrightarrow>\<^sub>A \<up> Q * true"
+  apply sep_auto
+  done
+
+lemma  set_fold_loop_correct:
+assumes "\<And> x y. <true>fimpl x y <\<lambda> r. \<up> (r = f x y)>"
+shows "<is_it S Simpl S' it> set_fold_loop it fimpl acc
+ <\<lambda>r. (\<exists>\<^sub>Axs. \<up> (set xs = S' \<and> r = foldl (\<lambda> x y. f y x) acc xs)) * is_set S Simpl>"
+proof(induction arbitrary: S' acc it rule: set_fold_loop.fixp_induct, goal_cases)
+  case 1
+  then show ?case by simp
+next
+  case 2
+  then show ?case by simp
+next
+  case (3 others S' acc)
+  show ?case
+    apply(rule ht_bind)
+     apply(rule it_has_next_rule)
+    subgoal for b
+      apply(cases b)
+      subgoal
+        apply(subst if_not_P)
+         apply simp
+        apply(rule ht_bind)
+         apply (cases "S' = {}")
+        apply simp
+        apply(rule ht_frame)
+         apply(rule it_next_rule)
+         apply simp
+        subgoal for x
+          apply(cases x)
+          subgoal for x it
+            apply simp
+            apply(rule ht_bind[of _ _ "\<lambda> r. \<up> (r = f x acc) * (is_it S Simpl (S' - {x}) it * \<up> (x \<in> S') * \<up> (S' \<noteq> {}))"])
+            subgoal 
+              apply(rule weaken_conditions_and_frame[OF _ _ assms(1), of _ "(is_it S Simpl (S' - {x}) it * \<up> (x \<in> S') * \<up> (S' \<noteq> {}))"])
+              by sep_auto
+            subgoal for xb
+              apply(rule weaken_conditions_and_frame[OF _ _ 3, of _ "\<up> (x \<in> S') * \<up> (S' \<noteq> {})*\<up> (xb = f x acc)" "S' - {x}"])
+              subgoal
+                by sep_auto
+              apply simp
+              apply(rule ent_ex_preI)
+              subgoal for r xs
+              apply(rule ent_ex_postI[of _ _ "x#xs"])
+               by sep_auto
+             done
+           done
+         done
+       done
+     subgoal
+       apply simp
+       apply(rule ht_cons_post[of _ _ 
+           "\<lambda>r. \<up> (r = acc) * (\<up> (S' = {})* is_set S Simpl)"])
+        apply(rule ht_cons_pre[OF _ ht_frame[OF ], of _ true])
+         by(sep_auto intro: quit_iteration)
+       done
+     done
+ qed
+
+lemma set_fold_correct:
+  assumes "\<And> x y. <true>fimpl x y <\<lambda> r. \<up> (r = f x y)>"
+  shows "<is_set S Simpl>
+          set_fold Simpl fimpl acc 
+         <\<lambda> r.(\<exists>\<^sub>A xs. \<up> (set xs = S \<and> r = foldl (\<lambda> x y. f y x) acc xs)) * is_set S Simpl>"
+  unfolding set_fold_def 
+  using set_fold_loop_correct[of fimpl f S Simpl S _ acc, OF assms] 
+ by (sep_auto intro: it_init_rule)
+
+
 end
 
 
